proofs/AllocFree.fst
@@ -1,0 +1,48 @@
+module AllocFree
+
+open IncSepLogicOne
+
+// Def del programa a verificar
+(*
+  x = alloc()
+  free(x)
+  *x = 1
+*)
+
+let post_alloc (s : state) : prop =
+  exists (l : loc) (v : value). 
+    s._3 == Ok /\ 
+    s._1 "x" == Loc l /\ 
+    l =!= 0 /\ 
+    points_to l v s
+
+let pre_free (s:state) : prop = 
+  s._3 == Ok /\ post_alloc s
+
+let post_free (s : state) : prop =
+  exists (v : value). 
+    s._3 == Ok /\
+    points_to_empty (eval_expr s (Var "x")) s /\
+    pre_free (s._1, override s._2 (eval_expr s (Var "x")) (Full v), Ok)
+
+let pre_store (s : state) : prop =
+  s._3 == Ok /\ post_free s
+
+let post_uaf_err (s : state) : prop =
+  s._3 == Er /\ 
+  points_to_empty (eval_expr s (Var "x")) s /\
+  pre_store (s._1, s._2, Ok)
+
+let prog_uaf=
+  (Alloc "x") `Seq`
+  ((Free (Var "x")) `Seq`
+  (Store (Var "x") (Const 1)))
+
+let proof_uaf : isl_triple emp prog_uaf post_uaf_err =
+  let p_alloc = ISL_Alloc1 "x" in
+  let p_free = ISL_Free (Var "x") in
+  let p_store = ISL_StoreEr (Var "x") (Const 1) in
+
+  let p_seq1 = ISL_Seq p_free p_store in
+  let p_seq2 = ISL_Seq p_alloc p_seq1 in
+  ISL_Consequence emp post_uaf_err p_seq2 () ()
