proofs/RandomLoop.fst
@@ -1,0 +1,169 @@
+module RandomLoop
+
+open IncSepLogicOne
+open FStar.Classical
+
+// Utils
+let ( ||| ) = Choice
+let enot (e : expr) : expr = Minus (Const 1) e
+let ge (x y : expr) : expr = enot (Lt x y)
+
+// Def del programa a verificar
+(*
+n := 1000000;
+i, j := 0;
+while (i <= n){
+  i++;
+  if (random()) j++;
+}
+assert  (j != n);
+*)
+
+let init_vars = 
+  Assign "n" (Const 1000000) `Seq`
+  (Assign "i" (Const 0) `Seq`
+  Assign "j" (Const 0))
+
+let loop_body =
+  Assume (Lt (Var "i") (Var "n")) `Seq`
+  (Assign "i" (Plus (Var "i") (Const 1)) `Seq`
+  (Assign "j" (Plus (Var "j") (Const 1)) ||| Skip))
+
+let assert_stmt =
+  Seq (Assume (Eq (Var "j") (Var "n"))) Error |||
+  Assume (enot (Eq (Var "j") (Var "n")))
+
+let prog1 =
+  (Seq init_vars
+       (Seq (Kleene loop_body)
+            (Seq (Assume (Eq (Var "i") (Var "n"))) assert_stmt)))
+
+// Estados y condiciones
+let pre_vacia : cond =
+  fun _ -> true
+
+let post_er_bug : cond =
+  fun (st, _, m) -> st "n" == Nat 1000000 /\ st "i" == Nat 1000000 /\ st "j" == Nat 1000000 /\ m == Er
+
+let mid_i (k : nat) : cond =
+  fun (st, _, m) -> k < 1000000 /\ st "n" == Nat 1000000 /\ st "i" == Nat (k + 1) /\ st "j" == Nat k /\ m == Ok
+
+let variant (n : nat) : cond = 
+  fun (st, _, m) -> n <= 1000000 /\ st "n" == Nat 1000000 /\ st "i" == Nat n /\ st "j" == Nat n /\ m == Ok
+
+let pre_assign (k : nat) : cond = 
+  fun s -> variant k s /\ eval_expr s (Lt (Var "i") (Var "n")) == 0
+
+let pre_assert : cond = 
+  fun s -> exists (k : nat). variant k s
+
+// Lemas auxiliares
+let lemma_p_i_consequence (k:nat) (s:state)
+  : Lemma (requires mid_i k s)
+          (ensures (let st, hp, m = s in
+                   exists st_init. pre_assign k (st_init, hp, m) /\
+                   st "i" == Nat (eval_expr (st_init, hp, m) (Plus (Var "i") (Const 1))) /\
+                   (forall y. y <> "i" ==> st y == st_init y) /\
+                   m == Ok)) =
+  let st, hp, m = s in
+  let st_init = override st "i" (Nat k) in
+  let s_init = (st_init, hp, m) in
+  assert (eval_expr s_init (Var "i") == k)
+
+let lemma_p_j_consequence (k:nat) (s:state)
+  : Lemma (requires variant (k + 1) s)
+          (ensures (let st, hp, m = s in
+                   exists st_init. mid_i k (st_init, hp, m) /\
+                   st "j" == Nat (eval_expr (st_init, hp, m) (Plus (Var "j") (Const 1))) /\
+                   (forall y. y <> "j" ==> st y == st_init y) /\
+                   m == Ok)) =
+  let st, hp, m = s in
+  let st_init = override st "j" (Nat k) in
+  let s_init = (st_init, hp, m) in
+  assert (eval_expr s_init (Var "j") == k)
+
+let proof_loop_step (k : nat) : isl_triple (variant k) loop_body (variant (k + 1)) =
+  let p_assumed = ISL_Assume #(variant k) (Lt (Var "i") (Var "n")) in
+
+  let p_i_raw = ISL_Assign #(pre_assign k) "i" (Plus (Var "i") (Const 1)) in
+  let _ = forall_intro (move_requires (lemma_p_i_consequence k)) in
+  let p_i = ISL_Consequence (pre_assign k) (mid_i k) p_i_raw () () in
+
+  let p_j_raw = ISL_Assign #(mid_i k) "j" (Plus (Var "j") (Const 1)) in
+  let _ = forall_intro (move_requires (lemma_p_j_consequence k)) in
+  let p_j_branch = ISL_Consequence (mid_i k) (variant (k + 1)) p_j_raw () () in
+  let p_j = ISL_ChoiceL p_j_branch in
+  let p_j' = 
+    ISL_Consequence (fun s -> s._3 == Ok /\ mid_i k s) (variant (k + 1)) p_j () ()
+  in
+  let p_ij = ISL_Seq p_i p_j' in
+
+  let expected_pre_ij (s:state) : prop = 
+    s._3 == Ok /\ (s._3 == Ok /\ variant k s /\ eval_expr s (Lt (Var "i") (Var "n")) == 0)
+  in
+  let expected_post_ij (s:state) : prop =
+    variant (k + 1) s \/ s._3 == Er /\ mid_i k s
+  in
+
+  let p_ij_adapted = ISL_Consequence 
+    expected_pre_ij 
+    expected_post_ij 
+    p_ij 
+    () () 
+  in
+  let p_raw = ISL_Seq p_assumed p_ij_adapted in
+  ISL_Consequence (variant k) (variant (k + 1)) p_raw () ()
+
+let lemma_kleene : isl_triple 
+  (fun s -> variant 0 s /\ s._3 == Ok) 
+  (Kleene loop_body) 
+  (fun s -> exists (k:nat). variant k s /\ (k == 0 ==> s._3 == Ok)) =
+  let step (n : nat) =
+    ISL_Consequence
+      (fun s -> variant n s /\ s._3 == Ok)
+      (variant (n + 1))
+      (proof_loop_step n)
+      () ()
+  in 
+  ISL_KleeneVariant #variant #loop_body step
+
+let mid_n (s : state) : prop =
+  s._3 == Ok /\ s._1 "n" == Nat 1000000
+
+// Demostraciones formales
+let proof_init : isl_triple pre_vacia init_vars (variant 0) =
+  let p_n_raw = ISL_Assign #pre_vacia "n" (Const 1000000) in
+  let p_n = ISL_Consequence pre_vacia mid_n p_n_raw () () in
+  
+  let p_i = ISL_Assign #_ "i" (Const 0) in
+  let p_j = ISL_Assign #_ "j" (Const 0) in
+
+  let p_ij = ISL_Seq p_i p_j in
+  let p_init = ISL_Seq p_n p_ij in
+
+  ISL_Consequence pre_vacia (variant 0) p_init () ()
+
+let proof_assert : isl_triple pre_assert (Seq (Assume (Eq (Var "i") (Var "n"))) assert_stmt) post_er_bug =
+  let p_exit_raw = ISL_Assume #pre_assert (Eq (Var "i") (Var "n")) in
+  let p_exit = ISL_Consequence pre_assert (variant 1000000) p_exit_raw () () in
+
+  let p_cond_err = ISL_Assume #(fun s -> s._3 == Ok /\ variant 1000000 s) (Eq (Var "j") (Var "n")) in
+  let p_err = ISL_Error #_ in
+  let p_branch_err = ISL_Seq p_cond_err p_err in
+
+  let p_assert = ISL_ChoiceL p_branch_err in
+  let p_raw = ISL_Seq p_exit p_assert in
+  ISL_Consequence pre_assert post_er_bug p_raw () ()
+
+let proof_prog1 : isl_triple pre_vacia prog1 post_er_bug =
+  let expected_pre_assert (s:state) : prop =
+    s._3 == Ok /\ (exists (k: nat). variant k s /\ (k == 0 ==> s._3 == Ok))
+  in
+  let adapted_assert = ISL_Consequence expected_pre_assert post_er_bug proof_assert () () in
+  let p_kleene_assert = ISL_Seq lemma_kleene adapted_assert in
+  let expected_pre_kleene (s:state) : prop =
+    s._3 == Ok /\ variant 0 s
+  in
+  let adapted_kleene_assert = ISL_Consequence expected_pre_kleene post_er_bug p_kleene_assert () () in
+  let triple_seq = proof_init `ISL_Seq` adapted_kleene_assert in
+  ISL_Consequence pre_vacia post_er_bug triple_seq () ()
